Implementation of Mixture Normal Density in NGBoost

Soumya Sahu

August 2020

1 Mixture Normal Density

Consider k normal distributions, where density of distribution j can be written as,

$$f_j(x;\theta_j,\sigma_j^2) = \frac{1}{\sqrt{2\pi}\sigma_j} exp(-\frac{(x-\theta_j)^2}{2\sigma_j^2}).$$

A random variable is said to have k-mixture normal density if the random variable follows jth normal distribution with probability α_j such that $\sum_{j=1}^k \alpha_j = 1$. So, the density of k-mixture normal can be written in the following form,

$$f(x, \theta) = \sum_{j=1}^{k-1} \alpha_j f_j(x; \theta_j, \sigma_j^2) + (1 - \sum_{j=1}^{k-1} \alpha_j) f_k(x; \theta_k, \sigma_k^2),$$

where, $\sigma_j > 0$, $0 < \alpha_j < 1$, $\sum_{j=1}^{k-1} \alpha_j < 1$ and $\boldsymbol{\theta} = (\theta_1, ..., \theta_k, \sigma_1, ..., \sigma_k, \alpha_1, ..., \alpha_{k-1})^T$, vector of independent parameters.

2 Reparameterization

Implementation of NGBoost requires the parameter space must be \mathbb{R}^d , where d is dimension of parameter space. We transform σ_j and α_j in the following way,

$$\sigma_j^{\star} = \log_e \sigma_j, \qquad j = 1, 2, ..., k \qquad \qquad \alpha_j^{\star} = \log_e \left(\frac{\alpha_j}{1 - \sum_{l=1}^{k-1} \alpha_l} \right), \qquad j = 1, 2, ..., k - 1.$$

Here, $\sigma_j^{\star} \in \mathbb{R}$ while $\sigma_j = exp(\sigma_j^{\star}) > 0$ for j = 1, 2, ..., k.

Also,
$$\alpha_j^{\star} \in \mathbb{R}$$
 while $\alpha_j = \frac{exp(\alpha_j^{\star})}{1+\sum\limits_{l=1}^{k-1} exp(\alpha_l^{\star})} < 1$ and most importantly $\sum\limits_{l=1}^{k-1} \alpha_j = \frac{\sum\limits_{l=1}^{k-1} exp(\alpha_l^{\star})}{1+\sum\limits_{l=1}^{k-1} exp(\alpha_l^{\star})} < 1$.
So, after reparameterization, $\boldsymbol{\theta}$ becomes $\boldsymbol{\theta}^{\star} = (\theta_1, ..., \theta_k, \sigma_1^{\star}, ..., \sigma_k^{\star}, \alpha_1^{\star}, ..., \alpha_{k-1}^{\star})^T$.

3 Computing Gradient w.r.t θ^{\star}

Assume that we have a sample of size n, where the response variable is denoted as $x_1, x_2, ..., x_n$. Using Kullback-Leibler divergence, the score function (w.r.t θ) can be defined as,

$$S(\boldsymbol{\theta}) = -\frac{1}{n} \sum_{i=1}^{n} log_e f(x_i, \boldsymbol{\theta}),$$

where, $f(x, \theta)$ is the density of k-mixture normal density, defined in section 1. So, the gradient vector w.r.t θ can be defined as,

$$\Delta S(\boldsymbol{\theta}) = \left(\frac{\delta S}{\delta \theta_1} \dots \frac{\delta S}{\delta \theta_k} \frac{\delta S}{\delta \sigma_1} \dots \frac{\delta S}{\delta \sigma_k} \frac{\delta S}{\delta \alpha}\right)^T,$$

where, $\frac{\delta S}{\delta \alpha} = \left(\frac{\delta S}{\delta \alpha_1} \dots \frac{\delta S}{\delta \alpha_{k-1}}\right)^T$.

$$\frac{\delta S}{\delta \theta_j} = -\frac{1}{n} \sum_{i=1}^n \frac{\alpha_j}{f(x_i, \theta)} \frac{\delta f_j(x_i)}{\delta \theta_j},$$

where,

$$\frac{\delta f_j(x)}{\delta \theta_j} = \frac{\delta f_j(x;\theta_j,\sigma_j^2)}{\delta \theta_j} = \frac{1}{\sqrt{2\pi}} \frac{(x-\theta_j)}{\sigma_j^3} exp(-\frac{(x-\theta_j)^2}{2\sigma_j^2}), \qquad j = 1, 2, ..., k,$$

and

$$\frac{\delta S}{\delta \sigma_j} = -\frac{1}{n} \sum_{i=1}^n \frac{\alpha_j}{f(x_i, \theta)} \frac{\delta f_j(x_i)}{\delta \sigma_j},$$

where,

$$\frac{\delta f_j(x)}{\delta \sigma_j} = \frac{\delta f_j(x;\theta_j,\sigma_j^2)}{\delta \sigma_j} = \frac{1}{\sqrt{2\pi}} \frac{(x-\theta_j)^4 - \sigma_j^2}{\sigma_j^4} exp(-\frac{(x-\theta_j)^2}{2\sigma_j^2}), \qquad j = 1, 2, ..., k.$$

and

$$\frac{\delta S}{\delta \alpha_j} = -\frac{1}{n} \sum_{i=1}^n \frac{(f_j(x_i) - f_k(x_i))}{f(x_i, \boldsymbol{\theta})}.$$

In above equations, $\alpha_k = 1 - \sum_{l=1}^{k-1} \alpha_l$.

Now to find gradient w.r.t θ^{\star} we need to compute $\frac{\delta S}{\delta \sigma_j^{\star}}$ and $\frac{\delta S}{\delta \alpha^{\star}}$.

$$\frac{\delta S}{\delta \sigma_j^{\star}} = \frac{\delta S}{\delta \sigma_j} \frac{\delta \sigma_j}{\delta \sigma_j^{\star}} = \frac{\delta S}{\delta \sigma_j} \sigma_j, \qquad j = 1, 2, ..., k.$$

and

$$\frac{\delta S}{\delta \boldsymbol{\alpha}^{\star}} = A(\boldsymbol{\alpha})^{-1} \frac{\delta S}{\delta \boldsymbol{\alpha}}$$

where, $A(\alpha)$ is a matrix of dimension $(k-1) \times (k-1)$ with diagonal elements,

$$\frac{\delta \alpha_j^{\star}}{\delta \alpha_j} = \frac{1}{\alpha_j} + \frac{1}{1 - \sum_{l=1}^{k-1} \alpha_l}, \qquad j = 1, 2, \dots, k-1$$

and off-diagonal elements,

$$\frac{\delta \alpha_j^{\star}}{\delta \alpha_m} = \frac{1}{1 - \sum_{l=1}^{k-1} \alpha_l}, \qquad j = 1, 2, \dots, k-1, \quad m \neq j.$$

So, $A(\alpha) = diag\{\frac{1}{\alpha_1}, \frac{1}{\alpha_2}, \dots, \frac{1}{\alpha_{k-1}}\} + \frac{1}{1-\sum\limits_{l=1}^{k-1} \alpha_l} \mathbf{1}\mathbf{1}^T$, where **1** is unit vector of length k-1.

So, the gradient vector w.r.t θ^{\star} can be written as,

$$\Delta S(\boldsymbol{\theta^{\star}}) = \left(\frac{\delta S}{\delta \theta_1} \dots \frac{\delta S}{\delta \theta_k} \frac{\delta S}{\delta \sigma_1^{\star}} \dots \frac{\delta S}{\delta \sigma_k^{\star}} \frac{\delta S}{\delta \boldsymbol{\alpha^{\star}}}\right)^T$$

We have derived $S(\theta^*)$ as a function of θ but we can make it a function of θ^* by replacing σ_i and α_j as a function of σ_i^* and α_j^* respectively using the derivations in section 2.

4 Computing Information Function

Information function w.r.t θ^{\star} can be defined as,

$$I(\boldsymbol{\theta}^{\star}) = E[(\Delta S(\boldsymbol{\theta}^{\star}; y))(\Delta S(\boldsymbol{\theta}^{\star}; y))^{T}],$$

where, $\Delta S(\theta^{\star}; y)$ is the gradient based on a single sample y from a k-mixture normal distribution.

Under regularity conditions (which are satisfied by mixture normal) E(.) can be approximated by sample average. Let, $y_1, y_2, ..., y_N$ be N independent samples generated from k-mixture normal distribution. Then $I(\theta^*)$ can be approximated by,

$$I(\hat{\boldsymbol{\theta}}^{\star}) = \frac{1}{N} \sum_{i=1}^{N} (\Delta S(\boldsymbol{\theta}^{\star}; y_i)) (\Delta S(\boldsymbol{\theta}^{\star}; y_i))^T.$$

I suggest N must be as large as 10000 for good approximation.

How to generate a sample of size N from k-mixture normal distribution Draw a random number r from 1 to k, where probability of drawing number i is α_i (i = 1, 2, ..., k) and generate a sample from *r*-th normal distribution $(N(\mu_r, \sigma_r^2))$. Replicate this *N* times to get *N* independent samples. Unfortunately, this process may be time consuming. So, we can use exchangeability property of iid samples. Generate $[N\alpha_i]$ many samples from $N(\mu_i, \sigma_i^2)$ for i = 1, 2, ..., k - 1 and generate rest from $N(\mu_k, \sigma_k^2)$ and combine them to get total of *N* samples generated from *k*-mixture normal distribution.

5 Parameter Initialization in NGBoost Algorithm

In NGBoost algorithm, initial value of θ^{\star} can be found as $argmin_{\theta^{\star}}S(\theta^{\star})$ which is same as the maximum likelihood estimate of θ^{\star} based on the assumption that marginal distribution of response variable x is also a mixture of normal distributions. We can use Fisher Scoring algorithm to solve this problem as we have calculated the information matrix.

Let, $\theta^{\star(0)}$ be the maximum likelihood estimate. So, we use the following iterative step,

$$\boldsymbol{\theta}_{m+1}^{\star(0)} = \boldsymbol{\theta}_{m}^{\star(0)} - I(\boldsymbol{\theta}_{m}^{\star(0)})^{-1} \Delta S(\boldsymbol{\theta}_{m}^{\star(0)})$$

until $||\boldsymbol{\theta}^{\star 0}_{m+1} - \boldsymbol{\theta}^{\star 0}_{m}||_{1} < \epsilon$. $||.||_{1}$ is L_{1} norm and ϵ can be set to any small number like 10^{-5} .

Now an interesting question can be what is a good choice of starting value of the Fisher Scoring algorithm, i.e. what is $\boldsymbol{\theta}_{0}^{\star(0)}$. We can perform K-means clustering where we fix the number of clusters as k and sample mean, sample standard deviation from each cluster can be taken as μ, σ values in $\boldsymbol{\theta}_{0}^{\star(0)}$. We can take sample proportion of each cluster as α values in $\boldsymbol{\theta}_{0}^{\star(0)}$.